failed to derive no confusion

lib/StlcDep.v
@@ -1,150 +1,12 @@
 Require Export Lambda.SimpleTypes.
+From Equations Require Import Equations.
 
 (** * Dependently Typed Lambda Calculus. *)
 
 (** Inspired by
     Programming Language Foundations in Agda. *)
 
-(** List helpers. *)
-
-Section List.
-  Context {A : Set}.
-
-  Fixpoint Has (a : A) (Γ : list A) : Set :=
-    match Γ with
-    | []    => Empty_set
-    | h :: Δ => ((h = a) + Has a Δ)%type
-    end.
-
-  Variant zilch : list A -> Prop := zilch_nil : zilch [].
-  
-  Definition lookup :
-    forall {Γ : list A} {n : nat},
-      n < length Γ -> A.
-  Proof.
-    refine
-      (fix F Γ n HnΓ :=
-         match Γ as Γ' return Γ = Γ' -> A with
-         | []
-           => fun HΓΓ' => _
-         | a :: Δ
-         => fun HΓΓ' =>
-             match n as n' return n = n' -> A with
-             | O   => fun _ => a
-             | S k => fun Hnn' => F Δ k _
-             end eq_refl
-         end eq_refl).
-    - inv HΓΓ'; cbn in *; lia.
-    - subst; cbn in *; lia.
-  Defined.
-  
-  (* Require Import Extraction.
-     Recursive Extraction lookup. *)
-
-  Definition length_nth_error' :
-    forall {l : list A} {n : nat},
-      n < length l -> { a | nth_error l n = Some a }.
-  Proof.
-    refine
-    (fix F l n Hnl :=
-       match
-         l as l'
-         return
-         l = l' -> { a | nth_error l n = Some a } with
-       | [] => fun H => _
-       | h :: t
-         => fun H =>
-             match
-               n as n'
-               return
-               n = n' -> { a | nth_error l n = Some a } with
-             | O
-               => fun _ => @exist _ _ h _
-             | S k
-               => fun Hnn' =>
-                   match F t k _ with
-                   | exist _ a' Hk => @exist _ _ a' _
-                   end
-             end eq_refl
-       end eq_refl); subst; cbn in *;
-      lia || reflexivity || assumption.
-  Defined.
-
-
-  Definition nth_error_lookup :
-    forall {Γ : list A} {n : nat} (H : n < length Γ),
-      nth_error Γ n = Some (lookup H).
-  Proof.
-    intro l; induction l as [| a l IHl];
-      intros [| n] H; cbn in *;
-        try lia; eauto using Lt.lt_S_n.
-  Defined.
-
-  Definition ext' : forall {Γ Δ},
-      (forall a, Has a Γ -> Has a Δ) ->
-      forall b a, Has a (b :: Γ) -> Has a (b :: Δ).
-  Proof.
-    refine
-      (fun l d f b a H =>
-         match l as l' return l = l' -> Has a (b :: d) with
-         | [] => fun Hl => inl _
-         | h :: t
-           => fun Hl =>
-               match H with
-               | inl Hh => inl Hh
-               | inr Ht => inr (f _ Ht)
-               end
-         end eq_refl); subst; cbn in *.
-    destruct H as [H | H]; subst; reflexivity || contradiction.
-  Defined.
-
-  Definition Has_nth_error : forall {Γ a},
-      Has a Γ -> { n | nth_error Γ n = Some a}.
-  Proof.
-    intro l; induction l as [| h t IHt];
-      intros a Hal; cbn in *; try contradiction.
-    destruct Hal as [Hha | Hat]; subst.
-    - refine (exist _ 0 _); reflexivity.
-    - apply IHt in Hat as [k Hk].
-      refine (exist _ (S k) _); assumption.
-  Defined.
-
-  Definition nth_error_Has : forall {Γ a n},
-      nth_error Γ n = Some a -> Has a Γ.
-  Proof.
-    intro l; induction l as [| h t IHt];
-      intros a [| n] Hnth; cbn in *; try discriminate.
-    - inv Hnth; left; reflexivity.
-    - apply IHt in Hnth; right; assumption.
-  Defined.
-
-  Definition nth_error_Has' : forall {Γ a},
-      {n | nth_error Γ n = Some a} -> Has a Γ.
-  Proof.
-    intros l a [n H]; exact (nth_error_Has H).
-  Defined.
-
-  Fail Definition nth_error_Has : forall {Γ a},
-      Has a Γ <-> {n | nth_error Γ n = Some a}.
-  
-  Definition ext : forall {Γ Δ : list A},
-      (forall a, {n | nth_error Γ n = Some a} ->
-              {k | nth_error Δ k = Some a}) ->
-      forall b a, {n | nth_error (b :: Γ) n = Some a} ->
-               {k | nth_error (b :: Δ) k = Some a}.
-  Proof.
-    intros l d f b a Hab.
-    apply Has_nth_error.
-    apply nth_error_Has' in Hab.
-    pose proof (fun a H => nth_error_Has' (f a (Has_nth_error H))) as H.
-    eauto using ext'.
-  Defined.
-End List.
-
 (** De Bruijn syntax. *)
-
-Declare Scope term_scope.
-Delimit Scope term_scope with term.
 
 Reserved Notation "Γ '⊢' τ" (at level 80, no associativity).
 
@@ -159,25 +21,28 @@ Inductive term (Γ : list type) : type -> Set :=
     Γ ⊢ τ → τ' ->
     Γ ⊢ τ ->
     Γ ⊢ τ'
-where "Γ '⊢' τ" := (term Γ τ) : term_scope.
+where "Γ '⊢' τ" := (term Γ τ) : type_scope.
+
+Derive Signature for term.
+Equations Derive NoConfusion NoConfusionHom Subterm for type.
+Equations Derive NoConfusion NoConfusionHom Subterm for term.
 
 Local Hint Constructors term : core.
 
 Definition term_of_id :
   forall {Γ : list type} (n : nat) (H : n < length Γ),
-    (Γ ⊢ lookup H)%term := ltac:(eauto using nth_error_lookup).
+    Γ ⊢ lookup H := ltac:(eauto using nth_error_lookup).
 
 Definition term_of_nth_error
-           {Γ τ} (H : {n | nth_error Γ n = Some τ})
-  : (Γ ⊢ τ)%term :=
+           {Γ τ} (H : {n | nth_error Γ n = Some τ}) : Γ ⊢ τ :=
   match H with
   | exist _ _ Hn => Id _ _ _ Hn
   end.
 
 Definition App_eq
            (Γ : list type) (τ ρ σ : type)
-           (t₁ : (Γ ⊢ τ → ρ)%term) (t₂ : (Γ ⊢ σ)%term)
-  : τ = σ -> (Γ ⊢ ρ)%term.
+           (t₁ : Γ ⊢ τ → ρ) (t₂ : Γ ⊢ σ)
+  : τ = σ -> Γ ⊢ ρ.
 Proof.
   intros H; subst; exact (App _ _ _ t₁ t₂).
 Defined.
@@ -186,13 +51,16 @@ Local Hint Resolve App_eq : core.
 
 Definition App_lookup
            (Γ : list type) (n : nat) (H : n < length Γ) (τ ρ : type)
-           (t₁ : (Γ ⊢ lookup H)%term) (t₂ : (Γ ⊢ τ)%term) :
-  lookup H = τ → ρ -> (Γ ⊢ ρ)%term.
+           (t₁ : Γ ⊢ lookup H) (t₂ : Γ ⊢ τ) :
+  lookup H = τ → ρ -> Γ ⊢ ρ.
 Proof.
   intros Heq; rewrite Heq in t₁; eauto using App.
 Defined.
 
 Local Hint Resolve App_lookup : core.
+
+Declare Scope term_scope.
+Delimit Scope term_scope with term.
 
 Notation "'ID' x"
   := (Id _ x _)
@@ -226,7 +94,7 @@ Fixpoint Rename
          {Γ Δ}
          (f: forall τ, {n | nth_error Γ n = Some τ} ->
                   {k | nth_error Δ k = Some τ})
-         {σ} (t: (Γ ⊢ σ)%term) : (Δ ⊢ σ)%term :=
+         {σ} (t: Γ ⊢ σ) : Δ ⊢ σ :=
   match t with
   | Id _ _ _ Hm     => term_of_nth_error (f _ (exist _ _ Hm))
   | Abs _ ρ _ t'    => (`λ Rename (ext f ρ) t')%term
@@ -234,8 +102,8 @@ Fixpoint Rename
   end.
 
 Definition exts' : forall {Γ Δ},
-    (forall τ, Has τ Γ -> (Δ ⊢ τ)%term) ->
-    forall {ρ σ}, Has σ (ρ :: Γ) -> (ρ :: Δ ⊢ σ)%term.
+    (forall τ, Has τ Γ -> Δ ⊢ τ) ->
+    forall {ρ σ}, Has σ (ρ :: Γ) -> ρ :: Δ ⊢ σ.
 Proof.
   cbn; intros Γ Δ f ρ σ [H | H]; subst.
   - refine (Id _ 0 _ _); reflexivity.
@@ -247,8 +115,8 @@ Proof.
 Defined.
 
 Definition exts : forall {Γ Δ},
-    (forall τ, {n | nth_error Γ n = Some τ} -> (Δ ⊢ τ)%term) ->
-    forall ρ σ, {k | nth_error (ρ :: Γ) k = Some σ} -> (ρ :: Δ ⊢ σ)%term.
+    (forall τ, {n | nth_error Γ n = Some τ} -> Δ ⊢ τ) ->
+    forall ρ σ, {k | nth_error (ρ :: Γ) k = Some σ} -> ρ :: Δ ⊢ σ.
 Proof.
   intros Γ Δ f ρ σ H.
   apply nth_error_Has' in H.
@@ -258,8 +126,8 @@ Defined.
 
 Fixpoint subs
          {Γ Δ}
-         (f : forall τ, {n | nth_error Γ n = Some τ} -> (Δ ⊢ τ)%term)
-         {σ} (t : (Γ ⊢ σ)%term) : (Δ ⊢ σ)%term :=
+         (f : forall τ, {n | nth_error Γ n = Some τ} -> Δ ⊢ τ)
+         {σ} (t : Γ ⊢ σ) : Δ ⊢ σ :=
   match t with
   | Id _ _ _ Hn => f _ (exist _ _ Hn)
   | Abs _ ρ _ t' => (`λ subs (exts f ρ) t')%term
@@ -268,8 +136,7 @@ Fixpoint subs
 
 Definition sub
            {Γ τ σ}
-           (body : (τ :: Γ ⊢ σ)%term) (arg : (Γ ⊢ τ)%term)
-  : (Γ ⊢ σ)%term.
+           (body : τ :: Γ ⊢ σ) (arg : Γ ⊢ τ) : Γ ⊢ σ.
 Proof.
   refine (subs _ body).
   intros ρ [n Hρ].
@@ -283,41 +150,39 @@ Notation "x '[[' y ']]'"
 
 Reserved Notation "x '-->' y" (at level 80, no associativity).
 
-Inductive bred {Γ} : forall {τ}, (Γ ⊢ τ)%term -> (Γ ⊢ τ)%term -> Prop :=
-| bred_bred τ τ' (t₁ : (τ :: Γ ⊢ τ')%term) t₂ :
+Inductive bred {Γ} : forall {τ}, Γ ⊢ τ -> Γ ⊢ τ -> Prop :=
+| bred_bred τ τ' (t₁ : τ :: Γ ⊢ τ') t₂ :
     ((`λ t₁) ⋅ t₂)%term --> (t₁ [[ t₂ ]])%term
-| bred_abs τ τ' (t t' : (τ :: Γ ⊢ τ')%term) :
+| bred_abs τ τ' (t t' : τ :: Γ ⊢ τ') :
     t -->  t' ->
     (`λ t)%term --> (`λ t')%term
-| bred_app_l τ τ' (t₁ t₁' : (Γ ⊢ τ → τ')%term) t₂ :
+| bred_app_l τ τ' (t₁ t₁' : Γ ⊢ τ → τ') t₂ :
     t₁ -->  t₁' ->
     (t₁ ⋅ t₂)%term -->  (t₁' ⋅ t₂)%term
-| bred_app_r τ τ' (t₁ : (Γ ⊢ τ → τ')%term) t₂ t₂' :
+| bred_app_r τ τ' (t₁ : Γ ⊢ τ → τ') t₂ t₂' :
     t₂ -->  t₂' ->
     (t₁ ⋅ t₂)%term -->  (t₁ ⋅ t₂')%term
 where "x '-->' y" := (bred x y) : type_scope.
 
 Local Hint Constructors bred : core.
 
-Variant value {Γ} : forall {τ}, (Γ ⊢ τ)%term -> Prop :=
-  Abs_value τ τ' (t : (τ :: Γ ⊢ τ')%term) : value (`λ t)%term.
+Variant value {Γ} : forall {τ}, Γ ⊢ τ -> Prop :=
+  Abs_value τ τ' (t : τ :: Γ ⊢ τ') : value (`λ t)%term.
 
-Lemma value_ex : forall Γ τ (t : (Γ ⊢ τ)%term),
+Lemma value_ex : forall Γ τ (t : Γ ⊢ τ),
     value t ->
-    exists ρ σ (bdy : (ρ :: Γ ⊢ σ)%term), t ~= (`λ bdy)%term.
+    exists ρ σ (bdy : ρ :: Γ ⊢ σ), t ~= (`λ bdy)%term.
 Proof.
   intros Γ τ t Hv; inv Hv; eauto.
 Qed.
 
 Local Hint Constructors value : core.
 
-Definition Type_of {A : Type} (_ : A) :  Type := A.
-
 Variant is_arrow : type -> Prop :=
   Is_Arrow τ σ : is_arrow (τ → σ).
 
 (** Without [dependent induction], still needs axiom [Streicher K]. *)
-Lemma canonical_forms' : forall Γ τ (t : (Γ ⊢ τ)%term),
+Lemma canonical_forms' : forall Γ τ (t : Γ ⊢ τ),
     zilch Γ -> is_arrow τ ->
     (forall t', ~ (t -->  t')) -> value t.
 Proof.
@@ -339,7 +204,7 @@ Qed.
 
 (* Print Assumptions canonical_forms'. *)
 
-Lemma canonical_forms : forall τ σ (t : ([] ⊢ τ → σ)%term),
+Lemma canonical_forms : forall τ σ (t : [] ⊢ τ → σ),
       (forall t', ~ (t -->  t')) ->
     exists body, t = (`λ body)%term.
 Proof.
@@ -352,7 +217,7 @@ Qed.
 (*Check eq_rect.*)
 (*Print Assumptions canonical_forms.*)
 
-Theorem Progress' : forall Γ τ (t : (Γ ⊢ τ)%term),
+Theorem Progress' : forall Γ τ (t : Γ ⊢ τ),
     zilch Γ ->
     value t \/ exists t', t --> t'.
 Proof.
@@ -369,7 +234,7 @@ Proof.
       subst; eauto.
 Qed.
 
-Theorem Progress : forall τ (t : ([] ⊢ τ)%term),
+Theorem Progress : forall τ (t : [] ⊢ τ),
     value t \/ exists t', t --> t'.
 Proof.
   Local Hint Constructors zilch : core.
